Validator/Learning/ImperativeCompress.lean
@@ -48,16 +48,16 @@ def derive [DecidableEq α] (g: Expr.Grammar μ α) (xs: Exprs μ α) (t: Hedge.
       | Except.error err => Except.error err
       | Except.ok dxs => Except.ok dxs
 
-def derivs [DecidableEq α] (g: Expr.Grammar μ α) (x: Expr μ α) (forest: Hedge α): Except String (Expr μ α) :=
+def derivs [DecidableEq α] (g: Expr.Grammar μ α) (x: Expr μ α) (hedge: Hedge α): Except String (Expr μ α) :=
   -- see foldLoop for an explanation of what List.foldM does.
-  let dxs := List.foldlM (derive g) [x] forest
+  let dxs := List.foldlM (derive g) [x] hedge
   match dxs with
   | Except.error err => Except.error err
   | Except.ok [dx] => Except.ok dx
   | Except.ok _ => Except.error "expected one expression"
 
-def validate [DecidableEq α] (g: Expr.Grammar μ α) (x: Expr μ α) (forest: Hedge α): Except String Bool :=
-  match derivs g x forest with
+def validate [DecidableEq α] (g: Expr.Grammar μ α) (x: Expr μ α) (hedge: Hedge α): Except String Bool :=
+  match derivs g x hedge with
   | Except.error err => Except.error err
   | Except.ok x' => Except.ok (Expr.nullable x')
 
